prim/prim_constants.v
@@ -1,0 +1,29 @@
+Require Export VST.floyd.proofauto.
+
+Definition size := 8 : Z.
+Definition inf := 2147483646 : Z.
+(* Int.max_signed - 1 *)
+
+Lemma size_eq: size = 8.
+Proof. auto. Qed.
+
+Lemma inf_eq: inf = 2147483646. 
+Proof. auto. Qed.
+
+Lemma size_rep': 0 < size <= Int.max_signed.
+Proof. compute; split; [trivial | inversion 1]. Qed.
+
+Lemma size_rep: 0 <= size <= Int.max_signed.
+Proof. pose proof size_rep'. lia. Qed.
+
+Lemma inf_rep: 0 <= inf <= Int.max_signed.
+Proof. compute; split; inversion 1. Qed.
+
+Lemma inf_repable: repable_signed inf.
+Proof.
+  unfold repable_signed. rewrite inf_eq.
+  compute; split; inversion 1.
+Qed.
+
+Global Opaque size.
+Global Opaque inf.
